Generalize proof over arbitrary balance factor

proof/bt.v
@@ -1,70 +1,88 @@
 Require Import Arith NPeano Omega.
 
-Definition balanced (a b : nat) := b < 4 * a /\ a < 4 * b.
+Definition balanced (k a b : nat) := b < k * a /\ a < k * b.
 
-Inductive lbst : nat -> Set :=
-  | Leaf : lbst 1
-  | Node (a b : nat) : balanced a b -> lbst a -> lbst b -> lbst (1 + a + b).
+Inductive lbst (k : nat) : nat -> Set :=
+  | Leaf : lbst k 1
+  | Node (a b : nat) : balanced k a b -> lbst k a -> lbst k b -> lbst k (1 + a + b).
 
-Theorem bounded_disbalance a b (node : lbst (1 + a + b)) bal (la : lbst a) (lb : lbst b) :
-  (node = Node a b bal la lb) -> (max a b) * 5 < (1 + a + b) * 4.
+Theorem balanced_kpos (k a b : nat) : balanced k a b -> k > 1.
+Proof.
+  intro H.
+  destruct H.
+
+  destruct k.
+  inversion H.
+  destruct k.
+
+  intuition.
+  intuition.
+Qed.
+
+Theorem bounded_disbalance k a b (node : lbst k (1 + a + b)) bal (la : lbst k a) (lb : lbst k b) :
+  (node = Node k a b bal la lb) -> (max a b) * (S k) < (1 + a + b) * k.
 Proof.
   intro H.
   inversion bal.
+  assert (k > 1). apply (balanced_kpos k a b bal).
    
-  destruct (lt_dec a b).
-  rewrite max_r; intuition.
-  rewrite max_l; intuition.
+  destruct (lt_dec a b);
+    [rewrite max_r | rewrite max_l];
+    intuition;
+    rewrite mult_comm; simpl;
+    rewrite mult_plus_distr_r, plus_assoc, (mult_comm b), (mult_comm a);
+    omega.
 Qed.
 
-Fixpoint depth {n} f (l : lbst n) : nat :=
+Fixpoint depth {k n} f (l : lbst k n) : nat :=
   match l with
   | Leaf => 0
   | Node _ _ _ l r => S (f (depth f l) (depth f r))
   end.
 
-Theorem bounded_step n n' d total 
+Theorem bounded_step k n n' d total 
   (Hn : n <= n')
-  (Htotal : n' * 5 < total * 4)
-  (Hd : 5 ^ d <= 4 ^ d * n)
-  : 5 ^ (S d) <= 4 ^ (S d) * total.
+  (Htotal : n' * (S k) < total * k)
+  (Hd : (S k) ^ d <= k ^ d * n)
+  : (S k) ^ (S d) <= k ^ (S d) * total.
 Proof.
   do 2 rewrite (pow_succ_r _ _ (le_0_n _)).
   rewrite <- mult_assoc.
 
   (* <= weakens ?! *)
-  assert ((4 ^ d) * (n' * 5) <= (4 ^ d) * (total * 4)).
+  assert ((k ^ d) * (n' * (S k)) <= (k ^ d) * (total * k)).
   apply mult_le_compat_l.
   intuition.
 
   rewrite <- Nat.mul_shuffle3.
-  apply (le_trans _ (4 ^ d * (n' * 5)) _); intuition.
+  apply (le_trans _ (k ^ d * (n' * (S k))) _); intuition.
   
   rewrite (mult_comm n').
   rewrite Nat.mul_shuffle3.
   apply mult_le_compat_l.
 
-  apply (le_trans _ (4 ^ d * n) _).
+  apply (le_trans _ (k ^ d * n) _).
   trivial.
   
   apply mult_le_compat_l; auto.
+  rewrite (mult_comm k). auto.
 Qed.
 
-Theorem bounded_max {n} (l : lbst n) : 5 ^ (depth max l) <= 4 ^ (depth max l) * n.
+Theorem bounded_max {k n} (l : lbst k n) : (S k) ^ (depth max l) <= k ^ (depth max l) * n.
 Proof.
   remember l.
   induction l.
   subst; compute; intuition.
 
-  assert ((max a b) * 5 < (1 + a + b) * 4).
-  apply (bounded_disbalance a b l0 b0 l1 l2 Heql0).
+  assert ((max a b) * (S k) < (1 + a + b) * k).
+  apply (bounded_disbalance k a b l0 b0 l1 l2 Heql0).
 
   rewrite Heql0.
   simpl (depth max _).
  
   destruct (lt_dec (depth max l1) (depth max l2)).
   * rewrite max_r; intuition.
-    apply (bounded_step b (max a b)); intuition.
+    apply (bounded_step k b (max a b)); intuition.
   * rewrite max_l; intuition.
-    apply (bounded_step a (max a b)); intuition.
+    apply (bounded_step k a (max a b)); intuition.
 Qed.
